Makefile
@@ -195,10 +195,9 @@ CLOSE=SmallstepClosed.v CompilerClosed.v
 CONCUR=MultiLibs.v CMulti.v AsmMulti.v \
        CallconvBig.v MultiSimBig.v \
        HCompBig.v \
-       InliningproofC.v	
-       # InjpAccoComp.v VCompBig.v \
-       # SimplLocalsproofC.v CminorgenproofC.v InliningproofC.v \
-       # Composition.v InjpAccoComp.v 
+       InjpAccoComp.v VCompBig.v \
+       SimplLocalsproofC.v CminorgenproofC.v InliningproofC.v \
+       Composition.v
 
 
 
